src/lib/poly/gemm/Kuiper.Poly.GEMM.TensorCore2D.KernelDesc.fst
@@ -2,7 +2,6 @@ module Kuiper.Poly.GEMM.TensorCore2D.KernelDesc
 
 #lang-pulse
 
-// #set-options "--split_queries always"
 #set-options "--z3rlimit 40"
 
 open Kuiper
@@ -115,6 +114,7 @@ fn setup
    tm tn tk
    wm wn : szp { constraints bm bn bk tm tn tk wm wn })
   (#_ : squash (bm /? rows))
+  (#_ : squash (bk /?+ shared))
   (#_ : squash (bn /? cols))
   (#_ : squash (SZ.fits (bm * bk) /\ SZ.fits (bk * bn)))
   (#_ : squash (aligned 16 (core gA)))
@@ -230,34 +230,112 @@ fn setup
 }
 
 ghost
-fn single_even_barrier_p_to_q
+fn bp_sharing_to_bp_exclusive
   (#et : Type0) {| sized et, has_vec_cpy et |}
-  (#rows #cols : szp)
+  (#rows #cols : pos)
+  (l : full_mlayout rows cols)
+  (sar : gpu_array et (rows * cols))
+  (em : ematrix et rows cols)
+  (nthr : pos)
+  (#_ : squash (chunk et /?+ cols))
+  (#_ : squash (chunk et * nthr /?+ (rows * cols)))
+  requires
+    forall+ (_tid : natlt nthr).
+      bp_sharing (from_array l sar) em nthr
+  ensures
+    forall+ (tid : natlt nthr).
+      bp_exclusive (from_array l sar) em nthr tid
+{
+  gpu_matrix_gather_n (from_array l sar) nthr;
+  split_matrix_into_strided_chunks (from_array l sar) nthr;
+  forevery_map
+    (fun tid -> own_strided_chunks (from_array l sar) em nthr tid)
+    (fun tid -> bp_exclusive (from_array l sar) em nthr tid)
+    fn tid { fold bp_exclusive (from_array l sar) em nthr tid; };
+}
+
+ghost
+fn bp_exclusive_to_bp_sharing
+  (#et : Type0) {| sized et, has_vec_cpy et |}
+  (#rows #cols : pos)
+  (l : full_mlayout rows cols)
+  (sar : gpu_array et (rows * cols))
+  (em : ematrix et rows cols)
+  (nthr : pos)
+  (#_ : squash (SZ.fits (mlayout_size l)))
+  requires
+    forall+ (tid : natlt nthr).
+      bp_exclusive (from_array l sar) em nthr tid
+  ensures
+    forall+ (_tid : natlt nthr).
+      bp_sharing (from_array l sar) em nthr
+{
+  join_matrix_from_strided_chunks (from_array l sar) nthr;
+  gpu_matrix_share_n (from_array l sar) nthr;
+}
+
+ghost
+fn bp_sharing_to_bp_exclusive_underspec
+  (#et : Type0) {| sized et, has_vec_cpy et |}
+  (#rows #cols : pos)
   (l : full_mlayout rows cols)
   (sar : gpu_array et (rows * cols))
   (nthr : pos)
   (#_ : squash (chunk et /?+ cols))
   (#_ : squash (chunk et * nthr /?+ (rows * cols)))
   requires
-    forall+ (tid : natlt nthr).
-      (exists* (x : ematrix _ _ _). (from_array l sar) |-> Frac (1.0R /. nthr) x)
+    forall+ (_tid : natlt nthr).
+      exists* em.
+        bp_sharing (from_array l sar) em nthr
   ensures
     forall+ (tid : natlt nthr).
-      live_strided_chunks (from_array l sar) nthr tid
+      exists* em.
+        bp_exclusive (from_array l sar) em nthr tid
 {
   gpu_matrix_gather_n_underspec (from_array l sar) nthr;
-  with em. assert (from_array l sar) |-> em;
+  with em. assert from_array l sar |-> em;
   split_matrix_into_strided_chunks (from_array l sar) nthr;
   forevery_map
     (fun tid -> own_strided_chunks (from_array l sar) em nthr tid)
-    (fun tid -> live_strided_chunks (from_array l sar) nthr tid)
-    fn tid { fold live_strided_chunks (from_array l sar) nthr tid; };
+    (fun tid -> exists* em. bp_exclusive (from_array l sar) em nthr tid)
+    fn tid { fold bp_exclusive (from_array l sar) em nthr tid; };
+}
+
+ghost
+fn bp_exclusive_to_bp_sharing_underspec
+  (#et : Type0) {| sized et, has_vec_cpy et |}
+  (#rows #cols : pos)
+  (l : full_mlayout rows cols)
+  (sar : gpu_array et (rows * cols))
+  (nthr : pos)
+  (#_ : squash (SZ.fits (mlayout_size l)))
+  requires
+    forall+ (tid : natlt nthr).
+      exists* em.
+        bp_exclusive (from_array l sar) em nthr tid
+  ensures
+    forall+ (_tid : natlt nthr).
+      exists* em.
+        bp_sharing (from_array l sar) em nthr
+{
+  join_matrix_from_strided_chunks_underspec (from_array l sar) nthr;
+  with em. assert from_array l sar |-> em;
+  gpu_matrix_share_n (from_array l sar) nthr;
+  forevery_map
+    (fun (tid : natlt nthr) -> from_array l sar |-> Frac (1.0R /. nthr) em)
+    (fun (tid : natlt nthr) -> exists* em. bp_sharing (from_array l sar) em nthr)
+    fn tid { fold bp_sharing (from_array l sar) em nthr; };
 }
 
 ghost
 fn even_barrier_p_to_q
   (#et : Type0) {| sized et, has_vec_cpy et |}
-  (#bm #bn #bk: szp)
+  (#rows #shared #cols : pos)
+  (eA : ematrix et rows shared)
+  (eB : ematrix et shared cols)
+  (#bm : pos{bm /?+ rows})
+  (#bk : pos{bk /?+ shared})
+  (#bn : pos{bn /?+ cols})
   (l1 : full_mlayout bm bk)
   (l2 : full_mlayout bk bn)
   (sar1 : gpu_array et (bm * bk))
@@ -269,87 +347,75 @@ fn even_barrier_p_to_q
   (#_ : squash (chunk et * nthr /?+ (bk * bn)))
   requires
     forall+ (tid : natlt nthr).
-      (exists* (x : ematrix _ _ _). (from_array l1 sar1) |-> Frac (recip nthr) x) **
-      (exists* (x : ematrix _ _ _). (from_array l2 sar2) |-> Frac (recip nthr) x)
+      (exists* em1. bp_sharing (from_array l1 sar1) em1 nthr) **
+      (exists* em2. bp_sharing (from_array l2 sar2) em2 nthr)
   ensures
     forall+ (tid : natlt nthr).
       live_strided_chunks (from_array l1 sar1) nthr tid **
       live_strided_chunks (from_array l2 sar2) nthr tid
 {
   forevery_unzip _ _;
-  single_even_barrier_p_to_q l1 sar1 nthr;
-  single_even_barrier_p_to_q l2 sar2 nthr;
+  bp_sharing_to_bp_exclusive_underspec l1 sar1 nthr;
+  bp_sharing_to_bp_exclusive_underspec l2 sar2 nthr;
   forevery_zip (fun (tid: natlt nthr) ->
       live_strided_chunks (from_array l1 sar1) nthr tid) _;
 }
 
 ghost
-fn single_odd_barrier_p_to_q
-  (#et : Type0) {| sized et, has_vec_cpy et |}
-  (#rows #cols : szp)
-  (l : full_mlayout rows cols)
-  (sar : gpu_array et (rows * cols))
-  (nthr : pos)
-  (#_ : squash (chunk et /?+ cols))
-  (#_ : squash (chunk et * nthr /?+ (rows * cols)))
-  (#_ : squash (SZ.fits (mlayout_size l)))
-  requires
-    forall+ (tid : natlt nthr). live_strided_chunks (from_array l sar) nthr tid
-  ensures
-    forall+ (tid : natlt nthr).
-      (exists* (em : ematrix _ _ _). (from_array l sar) |-> Frac (recip nthr) em)
-{
-  join_matrix_from_strided_chunks_underspec (from_array l sar) nthr;
-  with em. assert (from_array l sar) |-> em;
-  gpu_matrix_share_n (from_array l sar) nthr;
-  forevery_map
-    (fun (tid : natlt nthr) -> from_array l sar |-> Frac (recip nthr) em)
-    (fun (tid : natlt nthr) -> exists* (em : ematrix _ _ _). (from_array l sar) |-> Frac (recip nthr) em)
-    fn tid { (); };
-}
-
-ghost
 fn odd_barrier_p_to_q
   (#et : Type0) {| sized et, has_vec_cpy et |}
-  (#bm #bn #bk : szp)
+  (#rows #shared #cols : pos)
+  (eA : ematrix et rows shared)
+  (eB : ematrix et shared cols)
+  (#bm : pos{bm /?+ rows})
+  (#bk : pos{bk /?+ shared})
+  (#bn : pos{bn /?+ cols})
   (l1 : full_mlayout bm bk)
   (l2 : full_mlayout bk bn)
   (sar1 : gpu_array et (bm * bk))
   (sar2 : gpu_array et (bk * bn))
   (nthr : pos)
+  (bid : natlt (rows/bm * (cols/bn)))
+  (it : natlt (2 * (shared / bk)))
   (#_ : squash (chunk et /?+ bn))
   (#_ : squash (chunk et /?+ bk))
   (#_ : squash (chunk et * nthr /?+ (bm * bk)))
   (#_ : squash (chunk et * nthr /?+ (bk * bn)))
   (#_ : squash (SZ.fits (mlayout_size l1)))
   (#_ : squash (SZ.fits (mlayout_size l2)))
-requires
-  forall+ (tid : natlt nthr).
-    live_strided_chunks (from_array l1 sar1) nthr tid **
-    live_strided_chunks (from_array l2 sar2) nthr tid
-ensures
-  forall+ (tid : natlt nthr).
-    (exists* (x : ematrix _ _ _). (from_array l1 sar1) |-> Frac (recip nthr) x) **
-    (exists* (x : ematrix _ _ _). (from_array l2 sar2) |-> Frac (recip nthr) x)
+  requires
+    forall+ (tid : natlt nthr).
+      bp_exclusive (from_array l1 sar1) (ematrix_subtile eA bm bk (bid/(cols/bn)) (it/2)) nthr tid **
+      bp_exclusive (from_array l2 sar2) (ematrix_subtile eB bk bn (it/2) (bid%(cols/bn))) nthr tid
+  ensures
+    forall+ (tid : natlt nthr).
+      bp_sharing (from_array l1 sar1) (ematrix_subtile eA bm bk (bid/(cols/bn)) (it/2)) nthr **
+      bp_sharing (from_array l2 sar2) (ematrix_subtile eB bk bn (it/2) (bid%(cols/bn))) nthr
 {
   forevery_unzip _ _;
-  single_odd_barrier_p_to_q l1 sar1 nthr;
-  single_odd_barrier_p_to_q l2 sar2 nthr;
+  bp_exclusive_to_bp_sharing l1 sar1 _ nthr;
+  bp_exclusive_to_bp_sharing l2 sar2 _ nthr;
   forevery_zip
     (fun (tid : natlt nthr) ->
-      exists* (em: ematrix et (v bm) (v bk)).
-        (from_array l1 sar1) |-> Frac (recip nthr) em) _;
+      bp_sharing (from_array l1 sar1) (ematrix_subtile eA bm bk (bid/(cols/bn)) (it/2)) nthr)
+      _;
 }
 
 ghost
 fn barrier_p_to_q_transform
   (#et : Type0) {| sized et, has_vec_cpy et |}
-  (#bm #bn #bk : szp)
+  (#rows #shared #cols : pos)
+  (eA : ematrix et rows shared)
+  (eB : ematrix et shared cols)
+  (#bm : pos{bm /?+ rows})
+  (#bk : pos{bk /?+ shared})
+  (#bn : pos{bn /?+ cols})
   (l1 : full_mlayout bm bk)
   (l2 : full_mlayout bk bn)
   (sar1 : gpu_array et (bm * bk))
   (sar2 : gpu_array et (bk * bn))
   (nthr : pos)
+  (bid : natlt (rows/bm * (cols/bn)))
   (#_ : squash (chunk et /?+ bn))
   (#_ : squash (chunk et /?+ bk))
   (#_ : squash (chunk et * nthr /?+ (bm * bk)))
@@ -357,94 +423,93 @@ fn barrier_p_to_q_transform
   (#_ : squash (SZ.fits (mlayout_size l1)))
   (#_ : squash (SZ.fits (mlayout_size l2)))
   (it : nat)
-requires
-  forall+ (tid : natlt nthr). barrier_p (from_array l1 sar1) (from_array l2 sar2) nthr it tid
-ensures
-  forall+ (tid : natlt nthr). barrier_q (from_array l1 sar1) (from_array l2 sar2) nthr it tid
+  requires
+    forall+ (tid : natlt nthr).
+      barrier_p eA eB (from_array l1 sar1) (from_array l2 sar2) nthr bid it tid
+  ensures
+    forall+ (tid : natlt nthr).
+      barrier_q eA eB (from_array l1 sar1) (from_array l2 sar2) nthr bid it tid
 {
-  // if requires ANF
-  let ev = even it;
-  if ev {
-    ghost
-    fn evaux (tid : natlt nthr)
-      norewrite
-      requires
-        (barrier_p (from_array l1 sar1) (from_array l2 sar2) nthr) it tid
-      ensures
-        (exists* (x : ematrix _ _ _). (from_array l1 sar1) |-> Frac (1.0R /. nthr) x) **
-        (exists* (x : ematrix _ _ _). (from_array l2 sar2) |-> Frac (1.0R /. nthr) x)
-    {
-      rewrite barrier_p (from_array l1 sar1) (from_array l2 sar2) nthr it tid
-           as (exists* (x : ematrix _ _ _). (from_array l1 sar1) |-> Frac (1.0R /. nthr) x) **
-              (exists* (x : ematrix _ _ _). (from_array l2 sar2) |-> Frac (1.0R /. nthr) x);
-    };
-    forevery_map _ _ evaux;
-
-    even_barrier_p_to_q l1 l2 sar1 sar2 nthr;
-
-    ghost
-    fn evaux2 (tid : natlt nthr)
-    requires
-      live_strided_chunks (from_array l1 sar1) nthr tid **
-      live_strided_chunks (from_array l2 sar2) nthr tid
-    ensures
-      barrier_q (from_array l1 sar1) (from_array l2 sar2) nthr it tid
-    {
-      rewrite live_strided_chunks (from_array l1 sar1) nthr tid **
-              live_strided_chunks (from_array l2 sar2) nthr tid
-           as barrier_q (from_array l1 sar1) (from_array l2 sar2) nthr it tid;
-    };
-    forevery_map _ _ evaux2;
+  if (it >= 2 * (shared / bk)) {
+    forevery_map
+      (fun (tid : natlt nthr) ->
+        barrier_p eA eB (from_array l1 sar1) (from_array l2 sar2) nthr bid it tid)
+      (fun (tid : natlt nthr) ->
+        barrier_q eA eB (from_array l1 sar1) (from_array l2 sar2) nthr bid it tid)
+      fn tid {
+        rewrite barrier_p eA eB (from_array l1 sar1) (from_array l2 sar2) nthr bid it tid as emp;
+        rewrite emp as barrier_q eA eB (from_array l1 sar1) (from_array l2 sar2) nthr bid it tid;
+      };
   } else {
-    ghost
-    fn oddaux (tid : natlt nthr)
-      norewrite
-      requires
-        barrier_p (from_array l1 sar1) (from_array l2 sar2) nthr it tid
-      ensures
-        live_strided_chunks (from_array l1 sar1) nthr tid **
-        live_strided_chunks (from_array l2 sar2) nthr tid
-    {
-      rewrite barrier_p (from_array l1 sar1) (from_array l2 sar2) nthr it tid
-           as live_strided_chunks (from_array l1 sar1) nthr tid **
-              live_strided_chunks (from_array l2 sar2) nthr tid;
-    };
+    // if requires ANF
+    let ev = even it;
+    if ev {
+      assert pure (it < 2 * (shared / bk));
+      assert pure (even it);
+      forevery_map
+        (fun (tid : natlt nthr) ->
+          barrier_p eA eB (from_array l1 sar1) (from_array l2 sar2) nthr bid it tid)
+        (fun (tid : natlt nthr) ->
+          (exists* em1. bp_sharing (from_array l1 sar1) em1 nthr) **
+          (exists* em2. bp_sharing (from_array l2 sar2) em2 nthr)
+        )
+        fn tid {
+          rewrite barrier_p eA eB (from_array l1 sar1) (from_array l2 sar2) nthr bid it tid
+              as (exists* em1. bp_sharing (from_array l1 sar1) em1 nthr) **
+                  (exists* em2. bp_sharing (from_array l2 sar2) em2 nthr);
+        };
 
-    forevery_map _ _ oddaux;
-    odd_barrier_p_to_q l1 l2 sar1 sar2 nthr;
+      even_barrier_p_to_q eA eB l1 l2 sar1 sar2 nthr;
 
-    ghost
-    fn oddaux2 (tid : natlt nthr)
-      norewrite
-      requires
-        // explicit sizes are not helping
-        (exists* (x : ematrix et bm bk). (from_array l1 sar1) |-> Frac (recip nthr) x) **
-        (exists* (x : ematrix et bk bn). (from_array l2 sar2) |-> Frac (recip nthr) x)
-      ensures
-        barrier_q (from_array l1 sar1) (from_array l2 sar2) nthr it tid
-    {
-      // extra rewrite step reduces time for type checking by ~50%
-      rewrite
-          (exists* (x : ematrix _ _ _). (from_array l1 sar1) |-> Frac (recip nthr) x) **
-          (exists* (x : ematrix _ _ _). (from_array l2 sar2) |-> Frac (recip nthr) x)
-      as
-        (if even (it+1) then
-          (exists* (x : ematrix _ _ _). (from_array l1 sar1) |-> Frac (recip nthr) x) **
-          (exists* (x : ematrix _ _ _). (from_array l2 sar2) |-> Frac (recip nthr) x)
-        else
-          live_strided_chunks (from_array l1 sar1) nthr tid **
-          live_strided_chunks (from_array l2 sar2) nthr tid);
-      rewrite
-        (if even (it+1) then
-          (exists* (x : ematrix _ _ _). (from_array l1 sar1) |-> Frac (recip nthr) x) **
-          (exists* (x : ematrix _ _ _). (from_array l2 sar2) |-> Frac (recip nthr) x)
-        else
+      forevery_map
+        (fun (tid : natlt nthr) ->
           live_strided_chunks (from_array l1 sar1) nthr tid **
           live_strided_chunks (from_array l2 sar2) nthr tid)
-      as
-        barrier_q (from_array l1 sar1) (from_array l2 sar2) nthr it tid;
-    };
-    forevery_map _ _ oddaux2;
+        (fun (tid : natlt nthr) ->
+          barrier_q eA eB (from_array l1 sar1) (from_array l2 sar2) nthr bid it tid
+        )
+        fn tid {
+          rewrite
+            live_strided_chunks (from_array l1 sar1) nthr tid **
+            live_strided_chunks (from_array l2 sar2) nthr tid
+          as
+            barrier_q eA eB (from_array l1 sar1) (from_array l2 sar2) nthr bid it tid;
+        };
+    } else {
+      assert pure (it < 2 * (shared / bk));
+      assert pure (odd it);
+      forevery_map
+        (fun (tid : natlt nthr) ->
+          barrier_p eA eB (from_array l1 sar1) (from_array l2 sar2) nthr bid it tid)
+        (fun (tid : natlt nthr) ->
+          bp_exclusive (from_array l1 sar1) (ematrix_subtile eA bm bk (bid/(cols/bn)) (it/2)) nthr tid **
+          bp_exclusive (from_array l2 sar2) (ematrix_subtile eB bk bn (it/2) (bid%(cols/bn))) nthr tid
+        )
+        fn tid {
+          rewrite
+            barrier_p eA eB (from_array l1 sar1) (from_array l2 sar2) nthr bid it tid
+          as
+            bp_exclusive (from_array l1 sar1) (ematrix_subtile eA bm bk (bid/(cols/bn)) (it/2)) nthr tid **
+            bp_exclusive (from_array l2 sar2) (ematrix_subtile eB bk bn (it/2) (bid%(cols/bn))) nthr tid;
+        };
+
+      odd_barrier_p_to_q eA eB l1 l2 sar1 sar2 nthr bid it;
+
+      forevery_map
+        (fun (tid : natlt nthr) ->
+          bp_sharing (from_array l1 sar1) (ematrix_subtile eA bm bk (bid/(cols/bn)) (it/2)) nthr **
+          bp_sharing (from_array l2 sar2) (ematrix_subtile eB bk bn (it/2) (bid%(cols/bn))) nthr)
+        (fun (tid : natlt nthr) ->
+          barrier_q eA eB (from_array l1 sar1) (from_array l2 sar2) nthr bid it tid
+        )
+        fn tid {
+          rewrite
+            bp_sharing (from_array l1 sar1) (ematrix_subtile eA bm bk (bid/(cols/bn)) (it/2)) nthr **
+            bp_sharing (from_array l2 sar2) (ematrix_subtile eB bk bn (it/2) (bid%(cols/bn))) nthr
+          as
+            barrier_q eA eB (from_array l1 sar1) (from_array l2 sar2) nthr bid it tid;
+        };
+    }
   }
 }
 
@@ -468,6 +533,7 @@ fn block_setup
    tm tn tk
    wm wn : szp { constraints bm bn bk tm tn tk wm wn })
   (#_ : squash (bm /?+ rows))
+  (#_ : squash (bk /?+ shared))
   (#_ : squash (bn /?+ cols))
   (#_ : squash (SZ.fits (bm * bk) /\ SZ.fits (bk * bn)))
   (nblk : szp{SZ.v nblk == rows/bm * (cols/bn)})
@@ -524,7 +590,7 @@ fn block_setup
 
   (* create barrier token *)
   B.mk_barrier nthr _ _
-    (barrier_p_to_q_transform (R.row_major bm bk) (R.row_major bk bn) (fst sh) (fst (snd sh)) nthr);
+    (barrier_p_to_q_transform eA eB (R.row_major bm bk) (R.row_major bk bn) (fst sh) (fst (snd sh)) nthr bid);
   let sar1 = fst sh;
   let sar2 = fst (snd sh);
 
@@ -532,12 +598,12 @@ fn block_setup
   forevery_zip
     (fun tid -> exists* (x : seq et_ab). gpu_pts_to_array (fst (snd sh)) #(recip nthr) x)
     (fun tid ->
-      barrier_tok (R.row_major bm bk) (R.row_major bk bn) (fst sh) (fst (snd sh)) 0 nthr tid);
+      barrier_tok eA eB (R.row_major bm bk) (R.row_major bk bn) (fst sh) (fst (snd sh)) 0 nthr bid tid);
   forevery_zip
     (fun tid -> exists* (x : seq et_ab). gpu_pts_to_array (fst sh) #(recip nthr) x)
     (fun tid ->
       (exists* (x : seq et_ab). gpu_pts_to_array (fst (snd sh)) #(recip nthr) x) **
-      barrier_tok (R.row_major bm bk) (R.row_major bk bn) (fst sh) (fst (snd sh)) 0 nthr tid);
+      barrier_tok eA eB (R.row_major bm bk) (R.row_major bk bn) (fst sh) (fst (snd sh)) 0 nthr bid tid);
   forevery_zip #(natlt nthr)
     (fun tid -> kpre1 gA eA gB eB gC eC bm bn bk tm tn tk wm wn fA fB rA rB rC nthr bid tid) _;
   ()
@@ -562,6 +628,7 @@ fn block_teardown
    tm tn tk
    wm wn : szp { constraints bm bn bk tm tn tk wm wn })
   (#_ : squash (bm /?+ rows))
+  (#_ : squash (bk /?+ shared))
   (#_ : squash (bn /?+ cols))
   (#_ : squash (SZ.fits (bm * bk) /\ SZ.fits (bk * bn)))
   (nblk : szp{SZ.v nblk == rows/bm * (cols/bn)})
@@ -608,7 +675,7 @@ fn block_teardown
 
   drop_
     (forall+ (x: natlt nthr).
-      barrier_tok (R.row_major bm bk) (R.row_major bk bn) (fst sh) (fst (snd sh)) (2 * (shared/bk)) nthr x);
+      barrier_tok eA eB (R.row_major bm bk) (R.row_major bk bn) (fst sh) (fst (snd sh)) (2 * (shared/bk)) nthr bid x);
   ()
 }
 
@@ -707,6 +774,7 @@ fn teardown
    tm tn tk
    wm wn : szp { constraints bm bn bk tm tn tk wm wn })
   (#_ : squash (bm /?+ rows))
+  (#_ : squash (bk /?+ shared))
   (#_ : squash (bn /?+ cols))
   (#_ : squash (SZ.fits (bm * bk) /\ SZ.fits (bk * bn)))
   (nblk : szp{SZ.v nblk == rows/bm * (cols/bn)})
